src/heaplang/adequacy.v
@@ -1,13 +1,13 @@
 From ITree Require Import ITree Recursion RecursionFacts InterpFacts TranslateFacts Eqit.
 From iris Require Import invariants ghost_map.
 From iris.proofmode Require Import proofmode.
-From iris.itree Require Import wpi ub itree choice state later handler void heap.
+From iris.itree Require Import wpi ub itree choice state step handler void heap.
 From iris.itree.threadpool Require Import ctrace handler interleaving.
 From iris.itree.heaplang Require Import lang program_logic.
 
 (** An execution outcome of a HeapLang program. *)
 Definition Outcome R : Type :=
-  (heap.heap val * (R + last_thread_killed + ub_crash)) + later_exhausted.
+  (heap.heap val * (R + last_thread_killed + ub_crash)) + step_exhausted.
 (** An execution of a HeapLang program. *)
 Definition Execution R : Type :=
   itree voidE (Outcome R).
@@ -19,7 +19,7 @@ Definition heaplang_irel {R} (σ : heaplang_heap) (n : option nat) (t : itree he
     ub_irel t1 t2 ∧
     state_irel σ t2 t3 ∧
     demonic_irel t3 t4 ∧
-    later_irel n (insert_voidE t4) te.
+    step_irel n (insert_voidE t4) te.
 
 Definition heaplang_eval (e : expr) (σ : heaplang_heap) (n : option nat)
   (* TODO: Can remove the itree here? How would we represent diverging
@@ -30,7 +30,7 @@ Definition heaplang_eval (e : expr) (σ : heaplang_heap) (n : option nat)
 Definition relationally_adequate (n : option nat) (e : expr) (σ : heaplang_heap) (φ : val → Prop) : Prop :=
   ∀ te, heaplang_eval e σ n te → ∃ x, te ≈ Ret x ∧
     match x with
-    | inr LaterExhausted => is_Some n
+    | inr StepExhausted => is_Some n
     | inl (_, inr UbCrash) => False
     | inl (_, inl (inl v)) => φ v
     | inl (_, inl (inr _)) => True
@@ -48,11 +48,11 @@ that terminates returns a value satisfying [φ]. *)
 Definition partially_adequate (e : expr) (σ : heaplang_heap) (φ : val → Prop) : Prop :=
   ∀ n, relationally_adequate (Some n) e σ φ.
 
-(* FIXME: would be nice to have (put LaterE as the last event and prove
+(* FIXME: would be nice to have (put stepE as the last event and prove
           the following intermediate lemma)
-Lemma remove_timeout {R E} (t : itree (LaterE +' E) R) n r :
-  later_ifn n t ≈ Ret(inl r) →
-  later_ifn None t ≈ Ret(inl r).
+Lemma remove_timeout {R E} (t : itree (stepE +' E) R) n r :
+  step_ifn n t ≈ Ret(inl r) →
+  step_ifn None t ≈ Ret(inl r).
 Proof. ... Qed.
 Lemma totally_adequate_weaken {R} σ (t : itree heaplangE R) φ :
   totally_adequate σ t φ →
@@ -101,7 +101,7 @@ Section adequacy.
     WPi t @ heaplangH m; ⊤ {{ Φ }} -∗
     |={⊤, ∅}=> ∃ x, ⌜te ≈ Ret x⌝ ∗
       match x with
-      | inr LaterExhausted => ⌜is_Some n⌝
+      | inr StepExhausted => ⌜is_Some n⌝
       | inl (_, inr UbCrash) => |={∅, ⊤}=> False
       | inl (σ, inl (inl v)) => |={∅, ⊤}=> state_interp σ ∗ Φ v
       | inl (σ, inl (inr LastThreadKilled)) => |={∅, ⊤}=> state_interp σ
@@ -114,7 +114,7 @@ Section adequacy.
     iDestruct (demonic_adequacy with "Hwp") as "Hwp"; [done|].
     rewrite -wpi_clear_mask. iMod "Hwp".
     iDestruct (wpi_insert_voidE with "Hwp") as "Hwp".
-    iDestruct (later_adequacy_empty with "Hlc Hwp") as "Hwp".
+    iDestruct (step_adequacy_empty with "Hlc Hwp") as "Hwp".
     iApply void_adequacy_empty.
     iApply wpi_wand; last done.
     iIntros (?) "HΦ". repeat case_match; eauto.
@@ -129,7 +129,7 @@ Section adequacy.
     WP e @ m; ⊤ {{ Φ }} -∗
     |={⊤, ∅}=> ∃ x, ⌜te ≈ Ret x⌝ ∗
       match x with
-      | inr LaterExhausted => ⌜is_Some n⌝
+      | inr StepExhausted => ⌜is_Some n⌝
       | inl (_, inr UbCrash) => |={∅, ⊤}=> False
       | inl (σ, inl (inl v)) => |={∅, ⊤}=> state_interp σ ∗ Φ v
       | inl (σ, inl (inr LastThreadKilled)) => |={∅, ⊤}=> state_interp σ
@@ -190,7 +190,7 @@ Section trace.
 
   (** Extract a trace for the interpreted ITree. *)
   Definition interp_tr_heaplang σ n (tr : ctrace sequential_heaplangE R) : option (trace voidE (Outcome R)) :=
-    interp_tr_later n <$> (insert_voidE_tr <$> (interp_tr <$> (interp_tr_state σ (interp_tr_ub (sequencify tr))))).
+    interp_tr_step n <$> (insert_voidE_tr <$> (interp_tr <$> (interp_tr_state σ (interp_tr_ub (sequencify tr))))).
 
   (** Construct a relational interpretation from a trace. *)
   Lemma heaplang_trace (tr : ctrace sequential_heaplangE R) (t : itree heaplangE R) tr' σ n :
@@ -209,7 +209,7 @@ Section trace.
     clear Htr. destruct H as (t3&Hst&Htr).
     eapply demonic_trace in Htr as (t4&Hinst&Htr).
     apply insert_voidE_trace in Htr.
-    apply later_trace with (n := n) in Htr as (t5&Hlat&Htr).
+    apply step_trace with (n := n) in Htr as (t5&Hlat&Htr).
     exists t5. split; last done.
     by exists t1, t2, t3, t4.
   Qed.
